otbn_model/code/example_lemmas.dfy
@@ -121,19 +121,13 @@ module example_lemmas {
 			}
 		}
 
-		// calc == {
-		// 	w1;
-		// 	uint256_hwb(w1_g1, uint256_lh(wacc_g9 + p10 * QUARTER_BASE), false);
-		// }
+		lemma_uint256_hwb(0, w1_g1, w1, uint256_lh(wacc_g2 + p3 * QUARTER_BASE), uint256_lh(wacc_g9 + p10 * QUARTER_BASE));
 	}
 
-	lemma lemma_uint256_split(x: uint256)
-		ensures x == uint256_lh(x) + uint256_uh(x) * HALF_BASE;
-
-	lemma lemma_uint256_hwb(x1: uint256, x2: uint256, x3: uint256, a: uint128, b: uint128)
-		requires x2 == uint256_hwb(x1, a, true);
-		requires x3 == uint256_hwb(x2, b, false);
-		ensures x3 == a + b * HALF_BASE;
+	lemma lemma_uint256_hwb(x1: uint256, x2: uint256, x3: uint256, lo: uint128, hi: uint128)
+		requires x2 == uint256_hwb(x1, lo, true);
+		requires x3 == uint256_hwb(x2, hi, false);
+		ensures x3 == lo + hi * HALF_BASE;
 	{
 		calc == {
 			x3;
@@ -142,13 +136,20 @@ module example_lemmas {
 			}
 			uint256_lh(x3) + uint256_uh(x3) * HALF_BASE;
 			{
-				assert uint256_uh(x3) == b && uint256_lh(x3) == uint256_lh(x2);
+				assert uint256_uh(x3) == hi && uint256_lh(x3) == uint256_lh(x2);
 			}
-			uint256_lh(x2) + b * HALF_BASE;
+			uint256_lh(x2) + hi * HALF_BASE;
 			{
-				assert uint256_lh(x2) == a;
+				assert uint256_lh(x2) == lo;
 			}
-			a + b * HALF_BASE;
+			lo + hi * HALF_BASE;
 		}
+	}
+
+	lemma lemma_uint256_split(x: uint256)
+		ensures x == uint256_lh(x) + uint256_uh(x) * HALF_BASE;
+	{
+		reveal uint256_lh();
+		reveal uint256_uh();
 	}
 }
